

GD for linear reg

$$y_i = ax_i + b \quad i = 1, \dots, n$$

$$E(a, b) = \sum_i (y_i - ax_i - b)^2$$

$$a \leftarrow a - \eta \frac{\partial E}{\partial a}$$

$$\begin{aligned} \frac{\partial E}{\partial a} &= \frac{\partial}{\partial a} \sum_i (y_i - ax_i - b)^2 \\ &= -2 \sum_i (y_i - ax_i - b) x_i \end{aligned}$$

$$a \leftarrow a + 2\eta \sum_i (y_i - ax_i - b) x_i$$

$$b \leftarrow b - \eta \frac{\partial E}{\partial b}$$

$$\begin{aligned} \frac{\partial E}{\partial b} &= \frac{\partial}{\partial b} \sum_i (y_i - ax_i - b)^2 \\ &= -2 \sum_i (y_i - ax_i - b) \end{aligned}$$

$$b \leftarrow b + 2\eta \sum_i (y_i - ax_i - b)$$

Matrix Factorization Model:

$$\hat{Y} = UV^T$$

$$U = n_n \times K$$

$$V = n_m \times K$$

$$V^T = K \times n_m$$

$$\begin{bmatrix} \dots & \hat{y}_{ij} & \dots \end{bmatrix} = \begin{bmatrix} \dots & u_i & \dots \end{bmatrix} \begin{bmatrix} \vdots & \hat{v}_j & \vdots \end{bmatrix}$$

$$\hat{y}_{ij} = u_i \cdot v_j = (UV^T)_{ij} = \sum_s u_{is} v_{js}$$

Mask Matrix:

$$R_{ij} = \begin{cases} 0 & \text{if } y_{ij} \text{ was blank} \\ 1 & \text{if not} \end{cases}$$

$$N = \sum_{i,j} R_{ij}$$

$$\text{loss: } \mathcal{L}(U, V) = \frac{1}{N} \sum_{(i,j): R_{ij}=1} (y_{ij} - u_i \cdot v_j)^2$$

Grad Descent:

$$W \leftarrow W - \eta \frac{\partial E}{\partial W}$$

Will need to update the elements of

u_i & v_j :

$$\underline{u_i} = (\underline{u_{i1}}, \underline{u_{i2}}, \dots, \underline{u_{ik}}, \dots, \underline{u_{iK}})$$

$$\underline{v_j} = (v_{j1}, v_{j2}, \dots, v_{jk}, \dots, v_{jK})$$

i & l are user indices

Updating eq:

$$\rightarrow \frac{\partial E}{\partial \underline{u_{lk}}} = \frac{1}{N} \sum_{\underline{(ij): R_{ij}=1}} \frac{\partial}{\partial \underline{u_{lk}}} (\underline{y_{ij}} - \underline{\hat{y}_{ij}})^2$$

$$= \frac{1}{N} \cdot 2 \sum_{(\dots)} (\underline{y_{ij}} - \underline{\hat{y}_{ij}}) \left(\frac{\partial \underline{\hat{y}_{ij}}}{\partial \underline{u_{lk}}} \right)$$

Claim:

$$\frac{\partial \hat{y}_{ij}}{\partial u_{lk}} = \begin{cases} 0 & \text{if } l \neq i \\ v_{jk} & \text{if } l = i \end{cases}$$

EX: $K=2$

$$\hat{y}_{34} = u_{31}v_{41} + u_{32}v_{42}$$

If $l=5$, $k=1$, then

$$\frac{\partial \hat{y}_{34}}{\partial u_{51}} = \frac{\partial}{\partial u_{51}} (\underbrace{u_{31}}_{=0} \underbrace{v_{41}}_{=0} + u_{32} \underbrace{v_{42}}_{=0}) = 0$$

If $l=3$, then:

$$\frac{\partial \hat{y}_{34}}{\partial u_{31}} = \frac{\partial}{\partial u_{31}} (\underbrace{u_{31}}_{=1} \underbrace{v_{41}}_{=0} + u_{32} \underbrace{v_{42}}_{=0}) = v_{41}$$

Updating eq:

$$\begin{aligned}\rightarrow \frac{\partial E}{\partial u_{lk}} &= \frac{1}{N} \sum_{(i,j): R_{ij}=1} \frac{\partial}{\partial u_{lk}} (y_{ij} - \hat{y}_{ij})^2 \\ &= -\frac{1}{N} \cdot 2 \sum_{(i,j)} (y_{ij} - \hat{y}_{ij}) \left(\frac{\partial \hat{y}_{ij}}{\partial u_{lk}} \right) \\ &= -\frac{2}{N} \sum_{j: R_{ij}=1} (y_{ij} - \hat{y}_{ij}) (v_{jk})\end{aligned}$$

$$u_{lk} \leftarrow u_{lk} - \eta \frac{\partial E}{\partial u_{lk}}$$

$$u_{lk} \leftarrow u_{lk} - \eta \left(-\frac{2}{N} \sum_{j: R_{ij}=1} (y_{ij} - \hat{y}_{ij}) v_{jk} \right)$$

$$u_{lk} \leftarrow u_{lk} + \frac{2\eta}{N} \sum_{(j: R_{ij}=1)} (y_{ij} - \hat{y}_{ij}) v_{jk}$$

A similar derivation for v_{lk} gives

$$v_{lk} \leftarrow v_{lk} + \frac{2\eta}{N} \sum_{(i: R_{il}=1)} (y_{ij} - \hat{y}_{ij}) u_{ik}$$

Vectorizing the GD eq.: element-wise multiplication

$$\text{Define } \Delta = (Y - UV^T) \otimes R$$

$$\Delta_{ij} = (y_{ij} - u_i \cdot v_j) \cdot r_{ij}$$

Define the matrices:

$$\begin{aligned} \frac{\partial E}{\partial U} &:= \text{the matrix w/ elements } \partial E / \partial u_{ik} \\ &= \left[\frac{\partial E}{\partial u_{ik}} \right]_{i,k} \end{aligned}$$

$$\frac{\partial E}{\partial V} = \left[\frac{\partial E}{\partial v_{jk}} \right]_{j,k}$$

Claim:

$$\frac{\partial E}{\partial U} = -\frac{2}{N} \Delta V^T \quad \text{Q}$$

$$\frac{\partial E}{\partial V} = -\frac{2}{N} \Delta^T U. \quad \text{E}$$

Why? let's go element-by-element.

$$\left(\frac{\partial E}{\partial u}\right)_{ik} = \frac{\partial E}{\partial u_{ik}} = -\frac{2}{N} \sum_j \Delta_{ij} v_{jk}$$

$$= -\frac{2}{N} \sum_j (y_{ij} - u_i v_j) \cdot \hat{r}_{ij} v_{jk}$$

$$= -\frac{2}{N} \sum_{j: \hat{r}_{ij}=1} (y_{ij} - u_i v_j) v_{jk}$$